core/effect_interpolants.v
@@ -15,6 +15,7 @@ Require Import effect_simulations.
 Require Import effect_simulations_lemmas.
 
 Require Import pure.
+Require Import full_composition.
 Module Type EffectInterpolationAxioms.
 
 Parameter effect_interp_II: forall m1 m2 nu12 
@@ -26,7 +27,7 @@ Parameter effect_interp_II: forall m1 m2 nu12
                              (SMvalNu' : sm_valid nu' m1' m3')
                              (MemInjNu' : Mem.inject (as_inj nu') m1' m3')
                              (ExtIncr: extern_incr (compose_sm nu12 nu23) nu')
-                             (Pure: pure_comp_ext nu12 nu23 m1 m2)
+                             (*Pure: pure_comp_ext nu12 nu23 m1 m2*)
                              (SMV12: sm_valid nu12 m1 m2)
                              (SMV23: sm_valid nu23 m2 m3)
                              (UnchPrivSrc: Mem.unchanged_on (fun b ofs => locBlocksSrc (compose_sm nu12 nu23) b = true /\ 
@@ -41,10 +42,11 @@ Parameter effect_interp_II: forall m1 m2 nu12
                                          (forall b, frgnBlocksTgt nu12 b = true -> 
                                                     frgnBlocksSrc nu23 b = true))
                              (Norm12: forall b1 b2 d1, extern_of nu12 b1 = Some(b2, d1) ->
-                                             exists b3 d2, extern_of nu23 b2 = Some(b3, d2)),
+                                             exists b3 d2, extern_of nu23 b2 = Some(b3, d2))
+                             (full: full_ext nu12 nu23),
      exists m2', exists nu12', exists nu23', nu'=compose_sm nu12' nu23' /\
                              extern_incr nu12 nu12' /\ extern_incr nu23 nu23' /\
-                             pure_comp_ext nu12' nu23' m1' m2' /\
+                             (*pure_comp_ext nu12' nu23' m1' m2' /\*)
                              Mem.inject (as_inj nu12') m1' m2' /\ mem_forward m2 m2' /\
                              Mem.inject (as_inj nu23') m2' m3' /\
                              sm_valid nu12' m1' m2' /\ sm_valid nu23' m2' m3' /\
@@ -64,7 +66,7 @@ Parameter effect_interp_II: forall m1 m2 nu12
                               outside of interpolation, in the transitivioty proof:
                               Mem.unchanged_on (local_out_of_reach nu23 m2) m3 m3'*).
 
-(*The following lemma from mem_interpolation (pre- structured-injection! is used in the proof of
+(*(*The following lemma from mem_interpolation (pre- structured-injection! is used in the proof of
   Lemma initial_inject_split in effect_simulations_trans. Prior to reintegrating global environments,
   thta final two clauses asserted by this lemma were not needed in the proof of initial_inject_split.*)
 Parameter interpolate_II_strongHeqMKI: forall m1 m2 j12 (MInj12 : Mem.inject j12 m1 m2) m1'
@@ -87,7 +89,7 @@ Parameter interpolate_II_strongHeqMKI: forall m1 m2 j12 (MInj12 : Mem.inject j12
                    Mem.inject j12' m1' m2' /\ mem_forward m2 m2' /\ 
                    Mem.inject j23' m2' m3' /\
                    Mem.unchanged_on (loc_out_of_reach j12 m1) m2 m2' /\
-                   pure_composition j12' j23' m1' m2' /\
+                   (*pure_composition j12' j23' m1' m2' /\*)
                    Mem.unchanged_on (loc_unmapped j23) m2 m2' /\ 
                    Mem.unchanged_on (loc_out_of_reach j23 m2) m3 m3' /\
                    (forall b1 b2 ofs2, j12' b1 = Some(b2,ofs2) -> 
@@ -98,6 +100,6 @@ Parameter interpolate_II_strongHeqMKI: forall m1 m2 j12 (MInj12 : Mem.inject j12
                      (j23 b2 = Some (b3,ofs3)) \/
                      (b2 = Mem.nextblock m2 /\ j' (Mem.nextblock m1) = Some(b3,ofs3)) \/
                      (exists m, (b2 = Mem.nextblock m2 + m)%positive /\ 
-                            j' ((Mem.nextblock m1+m)%positive) = Some(b3,ofs3))).
+                            j' ((Mem.nextblock m1+m)%positive) = Some(b3,ofs3))).*)
 
 End EffectInterpolationAxioms.
