core/effect_interpolation_proofs.v
@@ -4,6 +4,6 @@ Require Import mem_interpolation_II.
 
 Module EffectInterpolations <: EffectInterpolationAxioms.
 Definition effect_interp_II := EFF_interp_II.
-Definition interpolate_II_strongHeqMKI:= interpolate_II_strongHeqMKI.
+(*Definition interpolate_II_strongHeqMKI:= interpolate_II_strongHeqMKI.*)
 End EffectInterpolations.
 
